Correction de bugs de dB dans Atoms.v, transfert vers Meta.v dB OK dans Atoms.v
git-svn-id: http://gasp.dev.regis-gianas.com/svn/trunk@38 403e655e-980a-47bd-8c60-1ee5348bb6b7

coq/Atoms.v
@@ -1,5 +1,6 @@
 Require Import List.
 Require Import Program.
+Require Import Peano_dec.
 
 Definition var := nat.
 
@@ -14,7 +15,7 @@ Definition arity_of_atom (a : atom_name) : list atom :=
   match a with
     | A => []   | B => []
     | C => [ A []]  | D => [A []; B []]
-    | E => [A []; C [1]]
+    | E => [A []; C [0]]
   end.
 
 Definition env := list atom.
@@ -26,36 +27,64 @@ Inductive list_nth {A} : nat -> list A -> A -> Prop :=
   list_nth (S m) (b :: tl) a
   .
 
-Inductive wt_atom (Γ : env) : atom -> Prop :=
-| Wt_atom A xs :
-  wt_atoms Γ xs (arity_of_atom A) ->
-  wt_atom Γ (A xs)
+Definition rename_var y x k := 
+  match y with
+    | 0 => x+k
+    | S n => n
+  end.
 
-with wt_atoms (Γ : env) : list var -> list atom -> Prop :=
-| Wt_atoms_nil :
-  wt_atoms Γ [] []
-| Wt_atoms_cons x xs a As :
-  list_nth x Γ a ->
-  wt_atom Γ a ->
-  wt_atoms Γ xs As ->
-  wt_atoms Γ (x :: xs) (a :: As)
-  .
+Fixpoint rename_vars xs x k : list var :=
+  match xs with
+    | [] => []
+    | y::xs => rename_var y x k :: rename_vars xs x k
+  end.
 
-Inductive wt_atom_list (Γ : env) : list atom -> Prop :=
-| Wt_atom_list_nil :
-  wt_atom_list Γ []
-| Wt_atom_list_cons a As :
-  wt_atom Γ a ->
-  wt_atom_list (a :: Γ) As ->
-  wt_atom_list Γ (a :: As)
+Fixpoint rename_env As x k : env :=
+  match As with
+    | [] => []
+    | Atom a xs :: As => 
+      Atom a (rename_vars xs x k) :: rename_env As x (S k)
+  end.
+
+Inductive env_chop : env -> nat -> env -> Prop :=
+| Env_chop_o Γ :
+  env_chop Γ 0 Γ
+| Env_chop_s n a Γ Γ' :
+  env_chop Γ n Γ' ->
+  env_chop (a :: Γ) (S n) Γ'
 .
 
-Hint Constructors atom_name atom list_nth wt_atom wt_atoms wt_atom_list.
+Inductive wt_atoms (Γ : env) : list var -> list atom -> Prop :=
+| Wt_atoms_nil :
+  wt_atoms Γ [] []
+| Wt_atoms_cons Γ' x xs As (A:atom_name) ys :
+  list_nth x Γ (A ys) ->
+  env_chop Γ (S x) Γ' ->
+  wt_atoms Γ' ys (arity_of_atom A) ->
+  wt_atoms Γ xs (rename_env As x 0) ->
+  wt_atoms Γ (x :: xs) (A ys :: As)
+
+with wt_atom_list (Γ : env) : list atom -> Prop :=
+| Wt_atom_list_nil :
+  wt_atom_list Γ []
+| Wt_atom_list_cons A xs As :
+  wt_atoms Γ xs (arity_of_atom A) ->
+  wt_atom_list (A xs :: Γ) (rename_env As (length Γ) 0) ->
+  wt_atom_list Γ (A xs :: As)
+.
+
+Hint Constructors list_nth env_chop wt_atoms
+  wt_atom_list : patch.
+
+Ltac p := simpl;
+  try apply Wt_atom_list_cons;
+    try eapply Wt_atoms_cons; progress eauto with patch || p.
+
+
+Lemma ex_wt_atom_list2 : wt_atom_list [B []; A []] [D [1;0]].
+  p.
+Qed.
 
 Lemma ex_wt_atom_list : wt_atom_list [] [A[]; C[0]; E[1;0]].
- apply Wt_atom_list_cons. auto.
- apply Wt_atom_list_cons. apply Wt_atom; simpl; auto.
- apply Wt_atom_list_cons. apply Wt_atom; simpl; auto.
- apply Wt_atoms_cons; auto.
- apply Wt_atoms_cons; auto.     (* pas possible, bug de dB *)
-Abort.
+  p. 
+Qed.
